proof/amd64/avx2/Keccak1600_array_avx2x4.ec
@@ -1,0 +1,1359 @@
+(******************************************************************************
+   Keccak1600_array_avx2x4.ec:
+
+   Correctness proof for the Keccak (fixed-sized) array based
+  absorb/squeeze 4-way AVX2 implementation
+
+
+
+******************************************************************************)
+
+require import List Real Distr Int IntDiv StdOrder Ring.
+
+import IntID IntOrder.
+
+from Jasmin require import JModel.
+from Jasmin require import JArray.
+
+from CryptoSpecs require import FIPS202_SHA3 FIPS202_SHA3_Spec.
+from CryptoSpecs require export Keccak1600_Spec Keccakf1600_Spec.
+
+from JazzEC require Jazz_avx2.
+
+from JazzEC require import WArray800.
+from JazzEC require import Array25.
+
+from CryptoSpecs require import JWordList.
+from CryptoSpecs require import FIPS202_Keccakf1600.
+from CryptoSpecs require import Keccakf1600_Spec.
+
+require import Keccakf1600_avx2x4 Keccak1600_avx2x4 Keccak1600_imem_avx2x4.
+
+op addstate_avx2x4 (st: W256.t Array25.t, l0 l1 l2 l3: W8.t list): W256.t Array25.t.
+
+
+abstract theory KeccakArrayAvx2x4.
+
+op aSIZE: int.
+axiom aSIZE_ge0: 0 <= aSIZE.
+axiom aSIZE_u64: aSIZE < W64.modulus.
+
+print Jazz_avx2.M.
+module type MParam = {
+  proc keccakf1600_avx2x4 (st:W256.t Array25.t) : W256.t Array25.t
+  proc state_init_avx2x4 (st: W256.t Array25.t) : W256.t Array25.t
+  proc addratebit_avx2x4 (st:W256.t Array25.t, rATE8:int) : W256.t Array25.t
+  proc _4u64x4_u256x4(y0 y1 y2 y3 : W256.t) :
+    W256.t * W256.t * W256.t * W256.t
+}.
+
+clone import PolyArray as A
+ with op size <- aSIZE
+      proof ge0_size by exact aSIZE_ge0.
+
+clone import WArray as WA
+ with op size <- aSIZE.
+
+
+module M(P: MParam) = {
+  proc __aread_subu64 (buf:W8.t A.t, offset:W64.t, dELTA:int, lEN:int,
+                       tRAIL:int) : int * int * int * W64.t = {
+    var w:W64.t;
+    var iLEN:int;
+    var t16:W64.t;
+    var t8:W64.t;
+    iLEN <- lEN;
+    if ((lEN <= 0)) {
+      w <- (W64.of_int (tRAIL %% 256));
+      tRAIL <- 0;
+    } else {
+      if ((8 <= lEN)) {
+        w <-
+        (get64_direct (WA.init8 (fun i => buf.[i]))
+        (W64.to_uint (offset + (W64.of_int dELTA))));
+        dELTA <- (dELTA + 8);
+        lEN <- (lEN - 8);
+      } else {
+        if ((4 <= lEN)) {
+          w <-
+          (zeroextu64
+          (get32_direct (WA.init8 (fun i => buf.[i]))
+          (W64.to_uint (offset + (W64.of_int dELTA)))));
+          dELTA <- (dELTA + 4);
+          lEN <- (lEN - 4);
+        } else {
+          w <- (W64.of_int 0);
+        }
+        if ((2 <= lEN)) {
+          t16 <-
+          (zeroextu64
+          (get16_direct (WA.init8 (fun i => buf.[i]))
+          (W64.to_uint (offset + (W64.of_int dELTA)))));
+          dELTA <- (dELTA + 2);
+          lEN <- (lEN - 2);
+        } else {
+          t16 <- (W64.of_int 0);
+        }
+        if (((1 <= lEN) \/ ((tRAIL %% 256) <> 0))) {
+          if ((1 <= lEN)) {
+            t8 <-
+            (zeroextu64
+            (get8_direct (WA.init8 (fun i => buf.[i]))
+            (W64.to_uint (offset + (W64.of_int dELTA)))));
+            if (((tRAIL %% 256) <> 0)) {
+              t8 <- (t8 `|` (W64.of_int (256 * (tRAIL %% 256))));
+            } else {
+              
+            }
+            dELTA <- (dELTA + 1);
+            lEN <- (lEN - 1);
+          } else {
+            t8 <- (W64.of_int (tRAIL %% 256));
+          }
+          tRAIL <- 0;
+          t8 <- (t8 `<<` (W8.of_int (8 * (2 * ((iLEN %/ 2) %% 2)))));
+          t16 <- (t16 `|` t8);
+        } else {
+          
+        }
+        t16 <- (t16 `<<` (W8.of_int (8 * (4 * ((iLEN %/ 4) %% 2)))));
+        w <- (w `|` t16);
+      }
+    }
+    return (dELTA, lEN, tRAIL, w);
+  }
+  proc __aread_bcast_4subu64 (buf:W8.t A.t, offset:W64.t, dELTA:int,
+                              lEN:int, tRAIL:int) : int * int * int * W256.t = {
+    var w:W256.t;
+    var t64:W64.t;
+    var t128:W128.t;
+    if (((lEN <= 0) /\ ((tRAIL %% 256) = 0))) {
+      w <- (set0_256);
+    } else {
+      if ((8 <= lEN)) {
+        w <-
+        (VPBROADCAST_4u64
+        (get64_direct (WA.init8 (fun i => buf.[i]))
+        (W64.to_uint (offset + (W64.of_int dELTA)))));
+        dELTA <- (dELTA + 8);
+        lEN <- (lEN - 8);
+      } else {
+        (dELTA, lEN, tRAIL, t64) <@ __aread_subu64 (buf, offset, dELTA, 
+        lEN, tRAIL);
+        t128 <- (zeroextu128 t64);
+        w <- (VPBROADCAST_4u64 (truncateu64 t128));
+      }
+    }
+    return (dELTA, lEN, tRAIL, w);
+  }
+  proc __aread_subu128 (buf:W8.t A.t, offset:W64.t, dELTA:int,
+                        lEN:int, tRAIL:int) : int * int * int * W128.t = {
+    var w:W128.t;
+    var t64:W64.t;
+    if (((lEN <= 0) /\ ((tRAIL %% 256) = 0))) {
+      w <- (set0_128);
+    } else {
+      if ((16 <= lEN)) {
+        w <-
+        (get128_direct (WA.init8 (fun i => buf.[i]))
+        (W64.to_uint (offset + (W64.of_int dELTA))));
+        dELTA <- (dELTA + 16);
+        lEN <- (lEN - 16);
+      } else {
+        if ((8 <= lEN)) {
+          w <-
+          (VMOV_64
+          (get64_direct (WA.init8 (fun i => buf.[i]))
+          (W64.to_uint (offset + (W64.of_int dELTA)))));
+          dELTA <- (dELTA + 8);
+          lEN <- (lEN - 8);
+          (dELTA, lEN, tRAIL, t64) <@ __aread_subu64 (buf, offset, dELTA,
+          lEN, tRAIL);
+          w <- (VPINSR_2u64 w t64 (W8.of_int 1));
+        } else {
+          (dELTA, lEN, tRAIL, t64) <@ __aread_subu64 (buf, offset, dELTA,
+          lEN, tRAIL);
+          w <- (zeroextu128 t64);
+        }
+      }
+    }
+    return (dELTA, lEN, tRAIL, w);
+  }
+  proc __aread_subu256 (buf:W8.t A.t, offset:W64.t, dELTA:int,
+                        lEN:int, tRAIL:int) : int * int * int * W256.t = {
+    var w:W256.t;
+    var t128_1:W128.t;
+    var t128_0:W128.t;
+    if (((lEN <= 0) /\ ((tRAIL %% 256) = 0))) {
+      w <- (set0_256);
+    } else {
+      if ((32 <= lEN)) {
+        w <-
+        (get256_direct (WA.init8 (fun i => buf.[i]))
+        (W64.to_uint (offset + (W64.of_int dELTA))));
+        dELTA <- (dELTA + 32);
+        lEN <- (lEN - 32);
+      } else {
+        if ((16 <= lEN)) {
+          t128_0 <-
+          (get128_direct (WA.init8 (fun i => buf.[i]))
+          (W64.to_uint (offset + (W64.of_int dELTA))));
+          dELTA <- (dELTA + 16);
+          lEN <- (lEN - 16);
+          (dELTA, lEN, tRAIL, t128_1) <@ __aread_subu128 (buf, offset, 
+          dELTA, lEN, tRAIL);
+          w <-
+          (W256.of_int
+          (((W128.to_uint t128_0) %% (2 ^ 128)) +
+          ((2 ^ 128) * (W128.to_uint t128_1))));
+        } else {
+          t128_1 <- (set0_128);
+          (dELTA, lEN, tRAIL, t128_0) <@ __aread_subu128 (buf, offset, 
+          dELTA, lEN, tRAIL);
+          w <-
+          (W256.of_int
+          (((W128.to_uint t128_0) %% (2 ^ 128)) +
+          ((2 ^ 128) * (W128.to_uint t128_1))));
+        }
+      }
+    }
+    return (dELTA, lEN, tRAIL, w);
+  }
+  proc __awrite_subu64 (buf:W8.t A.t, offset:W64.t, dELTA:int,
+                        lEN:int, w:W64.t) : W8.t A.t * int * int = {
+    
+    if ((0 < lEN)) {
+      if ((8 <= lEN)) {
+        buf <-
+        (A.init
+        (WA.get8
+        (WA.set64_direct (WA.init8 (fun i => buf.[i]))
+        (W64.to_uint (offset + (W64.of_int dELTA))) w)));
+        dELTA <- (dELTA + 8);
+        lEN <- (lEN - 8);
+      } else {
+        if ((4 <= lEN)) {
+          buf <-
+          (A.init
+          (WA.get8
+          (WA.set32_direct (WA.init8 (fun i => buf.[i]))
+          (W64.to_uint (offset + (W64.of_int dELTA))) (truncateu32 w))));
+          w <- (w `>>` (W8.of_int 32));
+          dELTA <- (dELTA + 4);
+          lEN <- (lEN - 4);
+        } else {
+          
+        }
+        if ((2 <= lEN)) {
+          buf <-
+          (A.init
+          (WA.get8
+          (WA.set16_direct (WA.init8 (fun i => buf.[i]))
+          (W64.to_uint (offset + (W64.of_int dELTA))) (truncateu16 w))));
+          w <- (w `>>` (W8.of_int 16));
+          dELTA <- (dELTA + 2);
+          lEN <- (lEN - 2);
+        } else {
+          
+        }
+        if ((1 <= lEN)) {
+          buf <-
+          (A.init
+          (WA.get8
+          (WA.set8_direct (WA.init8 (fun i => buf.[i]))
+          (W64.to_uint (offset + (W64.of_int dELTA))) (truncateu8 w))));
+          dELTA <- (dELTA + 1);
+          lEN <- (lEN - 1);
+        } else {
+          
+        }
+      }
+    } else {
+      
+    }
+    return (buf, dELTA, lEN);
+  }
+  proc __awrite_subu128 (buf:W8.t A.t, offset:W64.t, dELTA:int,
+                         lEN:int, w:W128.t) : W8.t A.t * int * int = {
+    var t64:W64.t;
+    if ((0 < lEN)) {
+      if ((16 <= lEN)) {
+        buf <-
+        (A.init
+        (WA.get8
+        (WA.set128_direct (WA.init8 (fun i => buf.[i]))
+        (W64.to_uint (offset + (W64.of_int dELTA))) w)));
+        dELTA <- (dELTA + 16);
+        lEN <- (lEN - 16);
+      } else {
+        if ((8 <= lEN)) {
+          buf <-
+          (A.init
+          (WA.get8
+          (WA.set64_direct (WA.init8 (fun i => buf.[i]))
+          (W64.to_uint (offset + (W64.of_int dELTA)))
+          (MOVV_64 (truncateu64 w)))));
+          dELTA <- (dELTA + 8);
+          lEN <- (lEN - 8);
+          w <- (VPUNPCKH_2u64 w w);
+        } else {
+          
+        }
+        t64 <- (truncateu64 w);
+        (buf, dELTA, lEN) <@ __awrite_subu64 (buf, offset, dELTA, lEN, t64);
+      }
+    } else {
+      
+    }
+    return (buf, dELTA, lEN);
+  }
+  proc __awrite_subu256 (buf:W8.t A.t, offset:W64.t, dELTA:int,
+                         lEN:int, w:W256.t) : W8.t A.t * int * int = {
+    var t128:W128.t;
+    if ((0 < lEN)) {
+      if ((32 <= lEN)) {
+        buf <-
+        (A.init
+        (WA.get8
+        (WA.set256_direct (WA.init8 (fun i => buf.[i]))
+        (W64.to_uint (offset + (W64.of_int dELTA))) w)));
+        dELTA <- (dELTA + 32);
+        lEN <- (lEN - 32);
+      } else {
+        t128 <- (truncateu128 w);
+        if ((16 <= lEN)) {
+          buf <-
+          (A.init
+          (WA.get8
+          (WA.set128_direct (WA.init8 (fun i => buf.[i]))
+          (W64.to_uint (offset + (W64.of_int dELTA))) t128)));
+          dELTA <- (dELTA + 16);
+          lEN <- (lEN - 16);
+          t128 <- (VEXTRACTI128 w (W8.of_int 1));
+        } else {
+          
+        }
+        (buf, dELTA, lEN) <@ __awrite_subu128 (buf, offset, dELTA, lEN,
+        t128);
+      }
+    } else {
+      
+    }
+    return (buf, dELTA, lEN);
+  }
+  proc __addstate_bcast_array_avx2x4 (st:W256.t Array25.t, aT:int,
+                                      buf:W8.t A.t, offset:W64.t,
+                                      lEN:int, tRAILB:int) : W256.t Array25.t *
+                                                             int * W64.t = {
+    var aLL:int;
+    var lO:int;
+    var at:W64.t;
+    var dELTA:int;
+    var t256:W256.t;
+    var  _0:int;
+    var  _1:int;
+    var  _2:int;
+    var  _3:int;
+    aLL <- (aT + lEN);
+    lO <- (aT %% 8);
+    at <- (W64.of_int (32 * (aT %/ 8)));
+    dELTA <- 0;
+    if ((0 < lO)) {
+      if (((lO + lEN) < 8)) {
+        if ((tRAILB <> 0)) {
+          aLL <- (aLL + 1);
+        } else {
+          
+        }
+        (dELTA,  _2, tRAILB, t256) <@ __aread_bcast_4subu64 (buf, offset,
+        dELTA, lEN, tRAILB);
+        t256 <- (VPSLL_4u64 t256 (W128.of_int (8 * lO)));
+        t256 <-
+        (t256 `^`
+        (get256_direct (WArray800.init256 (fun i => st.[i])) (W64.to_uint at)
+        ));
+        st <-
+        (Array25.init
+        (WArray800.get256
+        (WArray800.set256_direct (WArray800.init256 (fun i => st.[i]))
+        (W64.to_uint at) t256)));
+        lO <- 0;
+        aT <- 0;
+        lEN <- 0;
+      } else {
+        if ((8 <= lEN)) {
+          t256 <-
+          (VPBROADCAST_4u64
+          (get64_direct (WA.init8 (fun i => buf.[i]))
+          (W64.to_uint (offset + (W64.of_int dELTA)))));
+          dELTA <- (dELTA + (8 - lO));
+        } else {
+          (dELTA,  _0,  _1, t256) <@ __aread_bcast_4subu64 (buf, offset,
+          dELTA, (8 - lO), 0);
+        }
+        lEN <- (lEN - (8 - lO));
+        aT <- (aT + (8 - lO));
+        t256 <- (VPSLL_4u64 t256 (W128.of_int (8 * lO)));
+        t256 <-
+        (t256 `^`
+        (get256_direct (WArray800.init256 (fun i => st.[i])) (W64.to_uint at)
+        ));
+        st <-
+        (Array25.init
+        (WArray800.get256
+        (WArray800.set256_direct (WArray800.init256 (fun i => st.[i]))
+        (W64.to_uint at) t256)));
+        at <- (at + (W64.of_int 32));
+      }
+    } else {
+      
+    }
+    offset <- (offset + (W64.of_int dELTA));
+    dELTA <- 0;
+    if ((8 <= lEN)) {
+      while ((at \ult (W64.of_int ((32 * (aT %/ 8)) + (32 * (lEN %/ 8)))))) {
+        t256 <-
+        (VPBROADCAST_4u64
+        (get64_direct (WA.init8 (fun i => buf.[i]))
+        (W64.to_uint offset)));
+        offset <- (offset + (W64.of_int 8));
+        t256 <-
+        (t256 `^`
+        (get256_direct (WArray800.init256 (fun i => st.[i])) (W64.to_uint at)
+        ));
+        st <-
+        (Array25.init
+        (WArray800.get256
+        (WArray800.set256_direct (WArray800.init256 (fun i => st.[i]))
+        (W64.to_uint at) t256)));
+        at <- (at + (W64.of_int 32));
+      }
+      lEN <- ((aT + lEN) %% 8);
+    } else {
+      
+    }
+    lO <- ((aT + lEN) %% 8);
+    if (((0 < lO) \/ (tRAILB <> 0))) {
+      if ((tRAILB <> 0)) {
+        aLL <- (aLL + 1);
+      } else {
+        
+      }
+      (dELTA,  _3, tRAILB, t256) <@ __aread_bcast_4subu64 (buf, offset,
+      dELTA, lO, tRAILB);
+      offset <- (offset + (W64.of_int dELTA));
+      t256 <-
+      (t256 `^`
+      (get256_direct (WArray800.init256 (fun i => st.[i])) (W64.to_uint at)));
+      st <-
+      (Array25.init
+      (WArray800.get256
+      (WArray800.set256_direct (WArray800.init256 (fun i => st.[i]))
+      (W64.to_uint at) t256)));
+    } else {
+      
+    }
+    return (st, aLL, offset);
+  }
+  proc __absorb_bcast_array_avx2x4 (st:W256.t Array25.t, aT:int,
+                                    buf:W8.t A.t, offset:W64.t,
+                                    lEN:int, rATE8:int, tRAILB:int) : 
+  W256.t Array25.t * int * W64.t = {
+    var aLL:int;
+    var iTERS:int;
+    var i:W64.t;
+    var  _0:int;
+    var  _1:int;
+    aLL <- (aT + lEN);
+    if (((aT + lEN) < rATE8)) {
+      (st, aT, offset) <@ __addstate_bcast_array_avx2x4 (st, aT, buf, 
+      offset, lEN, tRAILB);
+      if ((tRAILB <> 0)) {
+        st <@ P.addratebit_avx2x4 (st, rATE8);
+      } else {
+        
+      }
+    } else {
+      if ((aT <> 0)) {
+        (st,  _0, offset) <@ __addstate_bcast_array_avx2x4 (st, aT, buf,
+        offset, (rATE8 - aT), 0);
+        lEN <- (lEN - (rATE8 - aT));
+        st <@ P.keccakf1600_avx2x4 (st);
+        aT <- 0;
+      } else {
+        
+      }
+      iTERS <- (lEN %/ rATE8);
+      i <- (W64.of_int 0);
+      while ((i \ult (W64.of_int iTERS))) {
+        (st,  _1, offset) <@ __addstate_bcast_array_avx2x4 (st, 0, buf,
+        offset, rATE8, 0);
+        st <@ P.keccakf1600_avx2x4 (st);
+        i <- (i + (W64.of_int 1));
+      }
+      lEN <- (aLL %% rATE8);
+      (st, aT, offset) <@ __addstate_bcast_array_avx2x4 (st, 0, buf, 
+      offset, lEN, tRAILB);
+      if ((tRAILB <> 0)) {
+        st <@ P.addratebit_avx2x4 (st, rATE8);
+      } else {
+        
+      }
+    }
+    return (st, aT, offset);
+  }
+  proc __addstate_array_avx2x4 (st:W256.t Array25.t, aT:int,
+                                buf0:W8.t A.t, buf1:W8.t A.t,
+                                buf2:W8.t A.t, buf3:W8.t A.t,
+                                offset:W64.t, lEN:int, tRAILB:int) : 
+  W256.t Array25.t * int * W64.t = {
+    var aLL:int;
+    var lO:int;
+    var at:W64.t;
+    var dELTA:int;
+    var t0:W64.t;
+    var t1:W64.t;
+    var t2:W64.t;
+    var t3:W64.t;
+    var t256_0:W256.t;
+    var t256_1:W256.t;
+    var t256_2:W256.t;
+    var t256_3:W256.t;
+    var  _0:int;
+    var  _1:int;
+    var  _2:int;
+    var  _3:int;
+    var  _4:int;
+    var  _5:int;
+    var  _6:int;
+    var  _7:int;
+    var  _8:int;
+    var  _9:int;
+    var  _10:int;
+    var  _11:int;
+    var  _12:int;
+    var  _13:int;
+    var  _14:int;
+    var  _15:int;
+    var  _16:int;
+    var  _17:int;
+    var  _18:int;
+    var  _19:int;
+    var  _20:int;
+    var  _21:int;
+    var  _22:int;
+    var  _23:int;
+    var  _24:int;
+    var  _25:int;
+    var  _26:int;
+    var  _27:int;
+    var  _28:int;
+    var  _29:int;
+    var  _30:int;
+    var  _31:int;
+    var  _32:int;
+    aLL <- (aT + lEN);
+    lO <- (aT %% 8);
+    at <- (W64.of_int (4 * (aT %/ 8)));
+    dELTA <- 0;
+    if ((0 < lO)) {
+      if (((lO + lEN) < 8)) {
+        if ((tRAILB <> 0)) {
+          aLL <- (aLL + 1);
+        } else {
+          
+        }
+        ( _11,  _12,  _13, t0) <@ __aread_subu64 (buf0, offset, dELTA, 
+        lEN, tRAILB);
+        ( _14,  _15,  _16, t1) <@ __aread_subu64 (buf1, offset, dELTA, 
+        lEN, tRAILB);
+        ( _17,  _18,  _19, t2) <@ __aread_subu64 (buf2, offset, dELTA, 
+        lEN, tRAILB);
+        (dELTA,  _20,  _21, t3) <@ __aread_subu64 (buf3, offset, dELTA, 
+        lEN, tRAILB);
+        t0 <- (t0 `<<` (W8.of_int (8 * lO)));
+        t0 <-
+        (t0 `^`
+        (get64 (WArray800.init256 (fun i => st.[i]))
+        (W64.to_uint (at + (W64.of_int 0)))));
+        st <-
+        (Array25.init
+        (WArray800.get256
+        (WArray800.set64 (WArray800.init256 (fun i => st.[i]))
+        (W64.to_uint (at + (W64.of_int 0))) t0)));
+        t1 <- (t1 `<<` (W8.of_int (8 * lO)));
+        t1 <-
+        (t1 `^`
+        (get64 (WArray800.init256 (fun i => st.[i]))
+        (W64.to_uint (at + (W64.of_int 1)))));
+        st <-
+        (Array25.init
+        (WArray800.get256
+        (WArray800.set64 (WArray800.init256 (fun i => st.[i]))
+        (W64.to_uint (at + (W64.of_int 1))) t1)));
+        t2 <- (t2 `<<` (W8.of_int (8 * lO)));
+        t2 <-
+        (t2 `^`
+        (get64 (WArray800.init256 (fun i => st.[i]))
+        (W64.to_uint (at + (W64.of_int 2)))));
+        st <-
+        (Array25.init
+        (WArray800.get256
+        (WArray800.set64 (WArray800.init256 (fun i => st.[i]))
+        (W64.to_uint (at + (W64.of_int 2))) t2)));
+        t3 <- (t3 `<<` (W8.of_int (8 * lO)));
+        t3 <-
+        (t3 `^`
+        (get64 (WArray800.init256 (fun i => st.[i]))
+        (W64.to_uint (at + (W64.of_int 3)))));
+        st <-
+        (Array25.init
+        (WArray800.get256
+        (WArray800.set64 (WArray800.init256 (fun i => st.[i]))
+        (W64.to_uint (at + (W64.of_int 3))) t3)));
+        lO <- 0;
+        aT <- 0;
+        lEN <- 0;
+        tRAILB <- 0;
+      } else {
+        if ((8 <= lEN)) {
+          t0 <-
+          (get64_direct (WA.init8 (fun i => buf0.[i]))
+          (W64.to_uint (offset + (W64.of_int dELTA))));
+          t1 <-
+          (get64_direct (WA.init8 (fun i => buf1.[i]))
+          (W64.to_uint (offset + (W64.of_int dELTA))));
+          t2 <-
+          (get64_direct (WA.init8 (fun i => buf2.[i]))
+          (W64.to_uint (offset + (W64.of_int dELTA))));
+          t3 <-
+          (get64_direct (WA.init8 (fun i => buf3.[i]))
+          (W64.to_uint (offset + (W64.of_int dELTA))));
+          offset <- (offset + (W64.of_int (8 - lO)));
+        } else {
+          ( _0,  _1,  _2, t0) <@ __aread_subu64 (buf0, offset, dELTA,
+          (8 - lO), tRAILB);
+          ( _3,  _4,  _5, t1) <@ __aread_subu64 (buf1, offset, dELTA,
+          (8 - lO), tRAILB);
+          ( _6,  _7,  _8, t2) <@ __aread_subu64 (buf2, offset, dELTA,
+          (8 - lO), tRAILB);
+          (dELTA,  _9,  _10, t3) <@ __aread_subu64 (buf3, offset, dELTA,
+          (8 - lO), tRAILB);
+        }
+        lEN <- (lEN - (8 - lO));
+        aT <- (aT + (8 - lO));
+        t0 <- (t0 `<<` (W8.of_int (8 * lO)));
+        t0 <-
+        (t0 `^`
+        (get64 (WArray800.init256 (fun i => st.[i]))
+        (W64.to_uint (at + (W64.of_int 0)))));
+        st <-
+        (Array25.init
+        (WArray800.get256
+        (WArray800.set64 (WArray800.init256 (fun i => st.[i]))
+        (W64.to_uint (at + (W64.of_int 0))) t0)));
+        t1 <- (t1 `<<` (W8.of_int (8 * lO)));
+        t1 <-
+        (t1 `^`
+        (get64 (WArray800.init256 (fun i => st.[i]))
+        (W64.to_uint (at + (W64.of_int 1)))));
+        st <-
+        (Array25.init
+        (WArray800.get256
+        (WArray800.set64 (WArray800.init256 (fun i => st.[i]))
+        (W64.to_uint (at + (W64.of_int 1))) t1)));
+        t2 <- (t2 `<<` (W8.of_int (8 * lO)));
+        t2 <-
+        (t2 `^`
+        (get64 (WArray800.init256 (fun i => st.[i]))
+        (W64.to_uint (at + (W64.of_int 2)))));
+        st <-
+        (Array25.init
+        (WArray800.get256
+        (WArray800.set64 (WArray800.init256 (fun i => st.[i]))
+        (W64.to_uint (at + (W64.of_int 2))) t2)));
+        t3 <- (t3 `<<` (W8.of_int (8 * lO)));
+        t3 <-
+        (t3 `^`
+        (get64 (WArray800.init256 (fun i => st.[i]))
+        (W64.to_uint (at + (W64.of_int 3)))));
+        st <-
+        (Array25.init
+        (WArray800.get256
+        (WArray800.set64 (WArray800.init256 (fun i => st.[i]))
+        (W64.to_uint (at + (W64.of_int 3))) t3)));
+        at <- (at + (W64.of_int 4));
+      }
+    } else {
+      
+    }
+    offset <- (offset + (W64.of_int dELTA));
+    dELTA <- 0;
+    if ((8 <= lEN)) {
+      while ((at \ult (W64.of_int ((4 * (aT %/ 8)) + (16 * (lEN %/ 32)))))) {
+        t256_0 <-
+        (get256_direct (WA.init8 (fun i => buf0.[i]))
+        (W64.to_uint offset));
+        t256_1 <-
+        (get256_direct (WA.init8 (fun i => buf1.[i]))
+        (W64.to_uint offset));
+        t256_2 <-
+        (get256_direct (WA.init8 (fun i => buf2.[i]))
+        (W64.to_uint offset));
+        t256_3 <-
+        (get256_direct (WA.init8 (fun i => buf3.[i]))
+        (W64.to_uint offset));
+        offset <- (offset + (W64.of_int 32));
+        (t256_0, t256_1, t256_2, t256_3) <@ P._4u64x4_u256x4 (t256_0, 
+        t256_1, t256_2, t256_3);
+        t256_0 <-
+        (t256_0 `^`
+        (get256_direct (WArray800.init256 (fun i => st.[i]))
+        (W64.to_uint ((W64.of_int 8) * at))));
+        st <-
+        (Array25.init
+        (WArray800.get256
+        (WArray800.set256_direct (WArray800.init256 (fun i => st.[i]))
+        (W64.to_uint ((W64.of_int 8) * at)) t256_0)));
+        t256_1 <-
+        (t256_1 `^`
+        (get256_direct (WArray800.init256 (fun i => st.[i]))
+        (W64.to_uint (((W64.of_int 8) * at) + (W64.of_int 32)))));
+        st <-
+        (Array25.init
+        (WArray800.get256
+        (WArray800.set256_direct (WArray800.init256 (fun i => st.[i]))
+        (W64.to_uint (((W64.of_int 8) * at) + (W64.of_int 32))) t256_1)));
+        t256_2 <-
+        (t256_2 `^`
+        (get256_direct (WArray800.init256 (fun i => st.[i]))
+        (W64.to_uint (((W64.of_int 8) * at) + (W64.of_int 64)))));
+        st <-
+        (Array25.init
+        (WArray800.get256
+        (WArray800.set256_direct (WArray800.init256 (fun i => st.[i]))
+        (W64.to_uint (((W64.of_int 8) * at) + (W64.of_int 64))) t256_2)));
+        t256_3 <-
+        (t256_3 `^`
+        (get256_direct (WArray800.init256 (fun i => st.[i]))
+        (W64.to_uint (((W64.of_int 8) * at) + (W64.of_int 96)))));
+        st <-
+        (Array25.init
+        (WArray800.get256
+        (WArray800.set256_direct (WArray800.init256 (fun i => st.[i]))
+        (W64.to_uint (((W64.of_int 8) * at) + (W64.of_int 96))) t256_3)));
+        at <- (at + (W64.of_int 16));
+      }
+      while ((at \ult (W64.of_int ((4 * (aT %/ 8)) + (4 * (lEN %/ 8)))))) {
+        t0 <-
+        (get64_direct (WA.init8 (fun i => buf0.[i]))
+        (W64.to_uint offset));
+        t0 <-
+        (t0 `^`
+        (get64 (WArray800.init256 (fun i => st.[i]))
+        (W64.to_uint (at + (W64.of_int 0)))));
+        st <-
+        (Array25.init
+        (WArray800.get256
+        (WArray800.set64 (WArray800.init256 (fun i => st.[i]))
+        (W64.to_uint (at + (W64.of_int 0))) t0)));
+        t1 <-
+        (get64_direct (WA.init8 (fun i => buf1.[i]))
+        (W64.to_uint offset));
+        t1 <-
+        (t1 `^`
+        (get64 (WArray800.init256 (fun i => st.[i]))
+        (W64.to_uint (at + (W64.of_int 1)))));
+        st <-
+        (Array25.init
+        (WArray800.get256
+        (WArray800.set64 (WArray800.init256 (fun i => st.[i]))
+        (W64.to_uint (at + (W64.of_int 1))) t1)));
+        t2 <-
+        (get64_direct (WA.init8 (fun i => buf2.[i]))
+        (W64.to_uint offset));
+        t2 <-
+        (t2 `^`
+        (get64 (WArray800.init256 (fun i => st.[i]))
+        (W64.to_uint (at + (W64.of_int 2)))));
+        st <-
+        (Array25.init
+        (WArray800.get256
+        (WArray800.set64 (WArray800.init256 (fun i => st.[i]))
+        (W64.to_uint (at + (W64.of_int 2))) t2)));
+        t3 <-
+        (get64_direct (WA.init8 (fun i => buf3.[i]))
+        (W64.to_uint offset));
+        offset <- (offset + (W64.of_int 8));
+        t3 <-
+        (t3 `^`
+        (get64 (WArray800.init256 (fun i => st.[i]))
+        (W64.to_uint (at + (W64.of_int 3)))));
+        st <-
+        (Array25.init
+        (WArray800.get256
+        (WArray800.set64 (WArray800.init256 (fun i => st.[i]))
+        (W64.to_uint (at + (W64.of_int 3))) t3)));
+        at <- (at + (W64.of_int 4));
+      }
+      lEN <- ((aT + lEN) %% 8);
+    } else {
+      
+    }
+    lO <- ((aT + lEN) %% 8);
+    if (((0 < lO) \/ (tRAILB <> 0))) {
+      ( _22,  _23,  _24, t0) <@ __aread_subu64 (buf0, offset, dELTA, 
+      lO, tRAILB);
+      ( _25,  _26,  _27, t1) <@ __aread_subu64 (buf1, offset, dELTA, 
+      lO, tRAILB);
+      ( _28,  _29,  _30, t2) <@ __aread_subu64 (buf2, offset, dELTA, 
+      lO, tRAILB);
+      (dELTA,  _31,  _32, t3) <@ __aread_subu64 (buf3, offset, dELTA, 
+      lO, tRAILB);
+      offset <- (offset + (W64.of_int dELTA));
+      if ((tRAILB <> 0)) {
+        aLL <- (aLL + 1);
+        tRAILB <- 0;
+      } else {
+        
+      }
+      t0 <-
+      (t0 `^`
+      (get64 (WArray800.init256 (fun i => st.[i]))
+      (W64.to_uint (at + (W64.of_int 0)))));
+      st <-
+      (Array25.init
+      (WArray800.get256
+      (WArray800.set64 (WArray800.init256 (fun i => st.[i]))
+      (W64.to_uint (at + (W64.of_int 0))) t0)));
+      t1 <-
+      (t1 `^`
+      (get64 (WArray800.init256 (fun i => st.[i]))
+      (W64.to_uint (at + (W64.of_int 1)))));
+      st <-
+      (Array25.init
+      (WArray800.get256
+      (WArray800.set64 (WArray800.init256 (fun i => st.[i]))
+      (W64.to_uint (at + (W64.of_int 1))) t1)));
+      t2 <-
+      (t2 `^`
+      (get64 (WArray800.init256 (fun i => st.[i]))
+      (W64.to_uint (at + (W64.of_int 2)))));
+      st <-
+      (Array25.init
+      (WArray800.get256
+      (WArray800.set64 (WArray800.init256 (fun i => st.[i]))
+      (W64.to_uint (at + (W64.of_int 2))) t2)));
+      t3 <-
+      (t3 `^`
+      (get64 (WArray800.init256 (fun i => st.[i]))
+      (W64.to_uint (at + (W64.of_int 3)))));
+      st <-
+      (Array25.init
+      (WArray800.get256
+      (WArray800.set64 (WArray800.init256 (fun i => st.[i]))
+      (W64.to_uint (at + (W64.of_int 3))) t3)));
+    } else {
+      
+    }
+    return (st, aLL, offset);
+  }
+  proc __absorb_array_avx2x4 (st:W256.t Array25.t, aT:int,
+                              buf0:W8.t A.t, buf1:W8.t A.t,
+                              buf2:W8.t A.t, buf3:W8.t A.t,
+                              offset:W64.t, lEN:int, rATE8:int, tRAILB:int) : 
+  W256.t Array25.t * int * W64.t = {
+    var aLL:int;
+    var iTERS:int;
+    var i:W64.t;
+    var  _0:int;
+    var  _1:int;
+    aLL <- (aT + lEN);
+    if (((aT + lEN) < rATE8)) {
+      (st, aT, offset) <@ __addstate_array_avx2x4 (st, aT, buf0, buf1, 
+      buf2, buf3, offset, lEN, tRAILB);
+      if ((tRAILB <> 0)) {
+        st <@ P.addratebit_avx2x4 (st, rATE8);
+      } else {
+        
+      }
+    } else {
+      if ((aT <> 0)) {
+        (st,  _0, offset) <@ __addstate_array_avx2x4 (st, aT, buf0, buf1,
+        buf2, buf3, offset, (rATE8 - aT), 0);
+        lEN <- (lEN - (rATE8 - aT));
+        st <@ P.keccakf1600_avx2x4 (st);
+        aT <- 0;
+      } else {
+        
+      }
+      iTERS <- (lEN %/ rATE8);
+      i <- (W64.of_int 0);
+      while ((i \ult (W64.of_int iTERS))) {
+        (st,  _1, offset) <@ __addstate_array_avx2x4 (st, 0, buf0, buf1,
+        buf2, buf3, offset, rATE8, 0);
+        st <@ P.keccakf1600_avx2x4 (st);
+        i <- (i + (W64.of_int 1));
+      }
+      lEN <- (aLL %% rATE8);
+      (st, aT, offset) <@ __addstate_array_avx2x4 (st, 0, buf0, buf1, 
+      buf2, buf3, offset, lEN, tRAILB);
+      if ((tRAILB <> 0)) {
+        st <@ P.addratebit_avx2x4 (st, rATE8);
+      } else {
+        
+      }
+    }
+    return (st, aT, offset);
+  }
+  proc __dumpstate_array_avx2x4 (buf0:W8.t A.t, buf1:W8.t A.t,
+                                 buf2:W8.t A.t, buf3:W8.t A.t,
+                                 offset:W64.t, lEN:int, st:W256.t Array25.t) : 
+  W8.t A.t * W8.t A.t * W8.t A.t * W8.t A.t *
+  W64.t = {
+    var i:W64.t;
+    var x0:W256.t;
+    var x1:W256.t;
+    var x2:W256.t;
+    var x3:W256.t;
+    var t0:W64.t;
+    var t1:W64.t;
+    var t2:W64.t;
+    var t3:W64.t;
+    var  _0:int;
+    var  _1:int;
+    var  _2:int;
+    var  _3:int;
+    var  _4:int;
+    var  _5:int;
+    var  _6:int;
+    var  _7:int;
+    i <- (W64.of_int 0);
+    while ((i \slt (W64.of_int (32 * (lEN %/ 32))))) {
+      x0 <-
+      (get256_direct (WArray800.init256 (fun i_0 => st.[i_0]))
+      (W64.to_uint (((W64.of_int 4) * i) + (W64.of_int (0 * 32)))));
+      x1 <-
+      (get256_direct (WArray800.init256 (fun i_0 => st.[i_0]))
+      (W64.to_uint (((W64.of_int 4) * i) + (W64.of_int (1 * 32)))));
+      x2 <-
+      (get256_direct (WArray800.init256 (fun i_0 => st.[i_0]))
+      (W64.to_uint (((W64.of_int 4) * i) + (W64.of_int (2 * 32)))));
+      x3 <-
+      (get256_direct (WArray800.init256 (fun i_0 => st.[i_0]))
+      (W64.to_uint (((W64.of_int 4) * i) + (W64.of_int (3 * 32)))));
+      i <- (i + (W64.of_int 32));
+      (x0, x1, x2, x3) <@ P._4u64x4_u256x4 (x0, x1, x2, x3);
+      buf0 <-
+      (A.init
+      (WA.get8
+      (WA.set256_direct (WA.init8 (fun i_0 => buf0.[i_0]))
+      (W64.to_uint offset) x0)));
+      buf1 <-
+      (A.init
+      (WA.get8
+      (WA.set256_direct (WA.init8 (fun i_0 => buf1.[i_0]))
+      (W64.to_uint offset) x1)));
+      buf2 <-
+      (A.init
+      (WA.get8
+      (WA.set256_direct (WA.init8 (fun i_0 => buf2.[i_0]))
+      (W64.to_uint offset) x2)));
+      buf3 <-
+      (A.init
+      (WA.get8
+      (WA.set256_direct (WA.init8 (fun i_0 => buf3.[i_0]))
+      (W64.to_uint offset) x3)));
+      offset <- (offset + (W64.of_int 32));
+    }
+    while ((i \slt (W64.of_int (8 * (lEN %/ 8))))) {
+      t0 <-
+      (get64_direct (WArray800.init256 (fun i_0 => st.[i_0]))
+      (W64.to_uint (((W64.of_int 4) * i) + (W64.of_int (0 * 8)))));
+      buf0 <-
+      (A.init
+      (WA.get8
+      (WA.set64_direct (WA.init8 (fun i_0 => buf0.[i_0]))
+      (W64.to_uint offset) t0)));
+      t1 <-
+      (get64_direct (WArray800.init256 (fun i_0 => st.[i_0]))
+      (W64.to_uint (((W64.of_int 4) * i) + (W64.of_int (1 * 8)))));
+      buf1 <-
+      (A.init
+      (WA.get8
+      (WA.set64_direct (WA.init8 (fun i_0 => buf1.[i_0]))
+      (W64.to_uint offset) t1)));
+      t2 <-
+      (get64_direct (WArray800.init256 (fun i_0 => st.[i_0]))
+      (W64.to_uint (((W64.of_int 4) * i) + (W64.of_int (2 * 8)))));
+      buf2 <-
+      (A.init
+      (WA.get8
+      (WA.set64_direct (WA.init8 (fun i_0 => buf2.[i_0]))
+      (W64.to_uint offset) t2)));
+      t3 <-
+      (get64_direct (WArray800.init256 (fun i_0 => st.[i_0]))
+      (W64.to_uint (((W64.of_int 4) * i) + (W64.of_int (3 * 8)))));
+      buf3 <-
+      (A.init
+      (WA.get8
+      (WA.set64_direct (WA.init8 (fun i_0 => buf3.[i_0]))
+      (W64.to_uint offset) t3)));
+      i <- (i + (W64.of_int 8));
+      offset <- (offset + (W64.of_int 8));
+    }
+    if ((0 < (lEN %% 8))) {
+      t0 <-
+      (get64_direct (WArray800.init256 (fun i_0 => st.[i_0]))
+      (W64.to_uint (((W64.of_int 4) * i) + (W64.of_int (0 * 8)))));
+      (buf0,  _0,  _1) <@ __awrite_subu64 (buf0, offset, 0, (lEN %% 8), t0);
+      t1 <-
+      (get64_direct (WArray800.init256 (fun i_0 => st.[i_0]))
+      (W64.to_uint (((W64.of_int 4) * i) + (W64.of_int (1 * 8)))));
+      (buf1,  _2,  _3) <@ __awrite_subu64 (buf1, offset, 0, (lEN %% 8), t1);
+      t2 <-
+      (get64_direct (WArray800.init256 (fun i_0 => st.[i_0]))
+      (W64.to_uint (((W64.of_int 4) * i) + (W64.of_int (2 * 8)))));
+      (buf2,  _4,  _5) <@ __awrite_subu64 (buf2, offset, 0, (lEN %% 8), t2);
+      t3 <-
+      (get64_direct (WArray800.init256 (fun i_0 => st.[i_0]))
+      (W64.to_uint (((W64.of_int 4) * i) + (W64.of_int (3 * 8)))));
+      (buf3,  _6,  _7) <@ __awrite_subu64 (buf3, offset, 0, (lEN %% 8), t3);
+      offset <- (offset + (W64.of_int (lEN %% 8)));
+    } else {
+      
+    }
+    return (buf0, buf1, buf2, buf3, offset);
+  }
+  proc __squeeze_array_avx2x4 (buf0:W8.t A.t, buf1:W8.t A.t,
+                               buf2:W8.t A.t, buf3:W8.t A.t,
+                               offset:W64.t, lEN:int, st:W256.t Array25.t,
+                               rATE8:int) : W8.t A.t *
+                                            W8.t A.t *
+                                            W8.t A.t *
+                                            W8.t A.t * W64.t *
+                                            W256.t Array25.t = {
+    var iTERS:int;
+    var lO:int;
+    var i:W64.t;
+    iTERS <- (lEN %/ rATE8);
+    lO <- (lEN %% rATE8);
+    if ((0 < lEN)) {
+      if ((0 < iTERS)) {
+        i <- (W64.of_int 0);
+        while ((i \ult (W64.of_int iTERS))) {
+          st <@ P.keccakf1600_avx2x4 (st);
+          (buf0, buf1, buf2, buf3, offset) <@ __dumpstate_array_avx2x4 (
+          buf0, buf1, buf2, buf3, offset, rATE8, st);
+          i <- (i + (W64.of_int 1));
+        }
+      } else {
+        
+      }
+      if ((0 < lO)) {
+        st <@ P.keccakf1600_avx2x4 (st);
+        (buf0, buf1, buf2, buf3, offset) <@ __dumpstate_array_avx2x4 (
+        buf0, buf1, buf2, buf3, offset, lO, st);
+      } else {
+        
+      }
+    } else {
+      
+    }
+    return (buf0, buf1, buf2, buf3, offset, st);
+  }
+}.
+
+
+(*
+   PARAMETER MODULE
+*)
+module P: MParam = {
+  proc keccakf1600_avx2x4 = Jazz_avx2.M._keccakf1600_avx2x4
+  proc state_init_avx2x4 = Jazz_avx2.M.__state_init_avx2x4
+  proc addratebit_avx2x4 = Jazz_avx2.M.__addratebit_avx2x4
+  proc _4u64x4_u256x4 = Jazz_avx2.M.__4u64x4_u256x4
+}.
+
+
+lemma  aread_subu64_ll: islossless M(P).__aread_subu64
+ by islossless.
+
+hoare aread_subu64_h _buf _off _dlt _len _trail:
+ M(P).__aread_subu64
+ : buf=_buf /\ offset=_off /\ dELTA=_dlt /\ lEN=_len /\ tRAIL=_trail
+ ==> res.`1 = _dlt + min (max 0 _len) 8
+  /\ res.`2 = _len - min (max 0 _len) 8
+  /\ res.`3 = (if _len < 8 then 0 else _trail)
+  /\ res.`4 = W8u8.pack8 (sub _buf (to_uint _off+_dlt) (min (max 0 _len) 8) ++ [W8.of_int _trail]).
+admitted.
+
+phoare aread_subu64_ph _buf _off _dlt _len _trail:
+ [ M(P).__aread_subu64
+ : buf=_buf /\ offset=_off /\ dELTA=_dlt /\ lEN=_len /\ tRAIL=_trail
+ ==> res.`1 = _dlt + min (max 0 _len) 8
+  /\ res.`2 = _len - min (max 0 _len) 8
+  /\ res.`3 = (if _len < 8 then 0 else _trail)
+  /\ res.`4 = W8u8.pack8 (sub _buf (to_uint _off+_dlt) (min (max 0 _len) 8) ++ [W8.of_int _trail])
+ ] = 1%r.
+proof.
+by conseq aread_subu64_ll (aread_subu64_h _buf _off _dlt _len _trail).
+qed.
+
+lemma  aread_subu128_ll: islossless M(P).__aread_subu128
+ by islossless.
+
+hoare aread_subu128_h _buf _off _dlt _len _trail:
+ M(P).__aread_subu128
+ : buf=_buf /\ offset=_off /\ dELTA=_dlt /\ lEN=_len /\ tRAIL=_trail
+ ==> res.`1 = _dlt + min (max 0 _len) 16
+  /\ res.`2 = _len - min (max 0 _len) 16
+  /\ res.`3 = (if _len < 16 then 0 else _trail)
+  /\ res.`4 = W16u8.pack16 (sub _buf (to_uint _off+_dlt) (min (max 0 _len) 16) ++ [W8.of_int _trail]).
+admitted.
+
+phoare aread_subu128_ph _buf _off _dlt _len _trail:
+ [ M(P).__aread_subu128
+ : buf=_buf /\ offset=_off /\ dELTA=_dlt /\ lEN=_len /\ tRAIL=_trail
+ ==> res.`1 = _dlt + min (max 0 _len) 16
+  /\ res.`2 = _len - min (max 0 _len) 16
+  /\ res.`3 = (if _len < 16 then 0 else _trail)
+  /\ res.`4 = W16u8.pack16 (sub _buf (to_uint _off+_dlt) (min (max 0 _len) 16) ++ [W8.of_int _trail])
+ ] = 1%r.
+proof.
+by conseq aread_subu128_ll (aread_subu128_h _buf _off _dlt _len _trail).
+qed.
+
+lemma  aread_subu256_ll: islossless M(P).__aread_subu256
+ by islossless.
+
+hoare aread_subu256_h _buf _off _dlt _len _trail:
+ M(P).__aread_subu256
+ : buf=_buf /\ offset=_off /\ dELTA=_dlt /\ lEN=_len /\ tRAIL=_trail
+ ==> res.`1 = _dlt + min (max 0 _len) 32
+  /\ res.`2 = _len - min (max 0 _len) 32
+  /\ res.`3 = (if _len < 32 then 0 else _trail)
+  /\ res.`4 = W32u8.pack32 (sub _buf (to_uint _off+_dlt) (min (max 0 _len) 32) ++ [W8.of_int _trail]).
+admitted.
+
+phoare aread_subu256_ph _buf _off _dlt _len _trail:
+ [ M(P).__aread_subu256
+ : buf=_buf /\ offset=_off /\ dELTA=_dlt /\ lEN=_len /\ tRAIL=_trail
+ ==> res.`1 = _dlt + min (max 0 _len) 32
+  /\ res.`2 = _len - min (max 0 _len) 32
+  /\ res.`3 = (if _len < 32 then 0 else _trail)
+  /\ res.`4 = W32u8.pack32 (sub _buf (to_uint _off+_dlt) (min (max 0 _len) 32) ++ [W8.of_int _trail])
+ ] = 1%r.
+proof.
+by conseq aread_subu256_ll (aread_subu256_h _buf _off _dlt _len _trail).
+qed.
+
+
+lemma awrite_subu64_ll: islossless M(P).__awrite_subu64
+ by islossless.
+
+hoare awrite_subu64_h _buf _off _dlt _len _w:
+ M(P).__awrite_subu64
+ : buf=_buf /\ offset=_off /\ dELTA=_dlt /\ lEN=_len
+ ==> res.`1 = A.fill (nth W8.zero (W8u8.to_list _w)) (to_uint _off + _dlt) (min (max 0 _len) 8) _buf
+  /\ res.`2 = _dlt + min (max 0 _len) 8
+  /\ res.`3 = _len - min (max 0 _len) 8.
+proof.
+admitted.
+
+phoare awrite_subu64_ph _buf _off _dlt _len _w:
+ [ M(P).__awrite_subu64
+ : buf=_buf /\ offset=_off /\ dELTA=_dlt /\ lEN=_len
+ ==> res.`1 = A.fill (nth W8.zero (W8u8.to_list _w)) (to_uint _off + _dlt) (min (max 0 _len) 8) _buf
+  /\ res.`2 = _dlt + min (max 0 _len) 8
+  /\ res.`3 = _len - min (max 0 _len) 8
+ ] = 1%r.
+proof.
+by conseq awrite_subu64_ll (awrite_subu64_h _buf _off _dlt _len _w).
+qed.
+
+lemma awrite_subu128_ll: islossless M(P).__awrite_subu128
+ by islossless.
+
+hoare awrite_subu128_h _buf _off _dlt _len _w:
+ M(P).__awrite_subu128
+ : buf=_buf /\ offset=_off /\ dELTA=_dlt /\ lEN=_len
+ ==> res.`1 = A.fill (nth W8.zero (W16u8.to_list _w)) (to_uint _off + _dlt) (min (max 0 _len) 16) _buf
+  /\ res.`2 = _dlt + min (max 0 _len) 16
+  /\ res.`3 = _len - min (max 0 _len) 16.
+proof.
+admitted.
+
+phoare awrite_subu128_ph _buf _off _dlt _len _w:
+ [ M(P).__awrite_subu128
+ : buf=_buf /\ offset=_off /\ dELTA=_dlt /\ lEN=_len
+ ==> res.`1 = A.fill (nth W8.zero (W16u8.to_list _w)) (to_uint _off + _dlt) (min (max 0 _len) 16) _buf
+  /\ res.`2 = _dlt + min (max 0 _len) 16
+  /\ res.`3 = _len - min (max 0 _len) 16
+ ] = 1%r.
+proof.
+by conseq awrite_subu128_ll (awrite_subu128_h _buf _off _dlt _len _w).
+qed.
+
+lemma awrite_subu256_ll: islossless M(P).__awrite_subu256
+ by islossless.
+
+hoare awrite_subu256_h _buf _off _dlt _len _w:
+ M(P).__awrite_subu256
+ : buf=_buf /\ offset=_off /\ dELTA=_dlt /\ lEN=_len
+ ==> res.`1 = A.fill (nth W8.zero (W32u8.to_list _w)) (to_uint _off + _dlt) (min (max 0 _len) 32) _buf
+  /\ res.`2 = _dlt + min (max 0 _len) 32
+  /\ res.`3 = _len - min (max 0 _len) 32.
+proof.
+admitted.
+
+phoare awrite_subu256_ph _buf _off _dlt _len _w:
+ [ M(P).__awrite_subu256
+ : buf=_buf /\ offset=_off /\ dELTA=_dlt /\ lEN=_len
+ ==> res.`1 = A.fill (nth W8.zero (W32u8.to_list _w)) (to_uint _off + _dlt) (min (max 0 _len) 32) _buf
+  /\ res.`2 = _dlt + min (max 0 _len) 32
+  /\ res.`3 = _len - min (max 0 _len) 32
+ ] = 1%r.
+proof.
+by conseq awrite_subu256_ll (awrite_subu256_h _buf _off _dlt _len _w).
+qed.
+
+(*
+   ONE-SHOT (FIXED-SIZE) MEMORY ABSORB
+   ===================================
+*)
+
+lemma addstate_array_avx2x4_ll: islossless M(P).__addstate_array_avx2x4.
+admitted.
+
+lemma addstate_bcast_array_avx2x4_ll: islossless M(P).__addstate_bcast_array_avx2x4.
+admitted.
+
+phoare absorb_array_avx2x4_ll:
+ [ M(P).__absorb_array_avx2x4
+ : 0 < rATE8 <= 200 /\ 0 <= lEN /\ to_uint offset + lEN <= aSIZE
+ ==> true
+ ] = 1%r.
+proof.
+proc.
+have L: forall x, x <= aSIZE => x < W64.modulus.
+ by move=> *; apply (ler_lt_trans aSIZE) => //; exact aSIZE_u64.
+admitted.
+(*
+hoare absorb_array_avx2x4_h _l0 _l1 _l2 _l3 _buf _off _len _r8 _tb:
+ M(P).__absorb_array_avx2x4
+ : aT=size _l %% _r8 /\ buf=_buf /\ offset=_off /\ lEN=_len /\ rATE8=_r8 /\ tRAILB=_tb
+ /\ pabsorb_spec_avx2x4 _r8 _l0 _l1 _l2 _l3 st
+ /\ 0 <= _len
+ /\ to_uint _off + _len < aSIZE
+ ==> if _tb <> 0
+     then res.`1 = ABSORB1600 (W8.of_int _tb) _r8 (_l ++ sub _buf (to_uint _off) _len)
+       /\ res.`3 = _off + W64.of_int (max 0 _len)
+     else pabsorb_spec_ref _r8 (_l ++ sub _buf (to_uint _off) _len) res.`1
+       /\ res.`2 = (size _l + _len) %% _r8
+       /\ res.`3 = _off + W64.of_int _len.
+proof.
+proc.
+admit.
+qed.
+*)
+phoare absorb_bcast_array_avx2x4_ll:
+ [ M(P).__absorb_bcast_array_avx2x4
+ : 0 < rATE8 <= 200 /\ 0 <= lEN /\ to_uint offset + lEN <= aSIZE
+ ==> true
+ ] = 1%r.
+proof.
+proc.
+have L: forall x, x <= aSIZE => x < W64.modulus.
+ by move=> *; apply (ler_lt_trans aSIZE) => //; exact aSIZE_u64.
+admitted.
+
+
+(*
+   ONE-SHOT (FIXED-SIZE) MEMORY SQUEEZE
+   ====================================
+*)
+
+phoare dumpstate_array_avx2x4_ll: 
+ [ M(P).__dumpstate_array_avx2x4
+ : 0 <= lEN <= 200
+ ==> true
+ ] = 1%r.
+proof.
+proc => /=.
+admit(*
+seq 2: true => //.
+ while (#pre /\ 0 <= to_sint i <= lEN%/8) (lEN %/ 8 - to_sint i).
+  move=> z; auto => /> &m; rewrite sltE /= => Hlen0 Hlen1 Hi0 _.
+  rewrite of_sintK /smod ifF 1:/# modz_small 1:/# => Hi1.
+  have E: to_sint W64.one = 1 by rewrite to_sintE /smod.
+  do split. 
+  + by rewrite to_sintD_small E /#.
+  + by rewrite to_sintD_small E /#.
+  + by rewrite to_sintD_small E /#.
+ auto => /> &m; rewrite to_sintE /= => *.
+ split.
+  by rewrite /smod /= /#.
+ by move=> i ???; rewrite sltE of_sintK /smod ifF 1:/# modz_small 1:/# /#.
+by islossless.
+*).
+qed.
+
+(*
+hoare dumpstate_array_avx2_h _buf _off _len _st:
+ M(P).__dumpstate_array_avx2
+ : buf=_buf /\ offset=_off /\ lEN=_len /\ st=_st
+ /\ 0 <= _len <= 200
+ /\ to_uint _off + _len <= aSIZE
+ ==> res.`1 = A.fill (fun i=> (stbytes (stavx2_to_st25 _st)).[i-to_uint _off]) (to_uint _off) _len _buf
+  /\ res.`2 = _off + W64.of_int _len.
+admitted.
+
+phoare dumpstate_array_avx2_ph _buf _off _len _st:
+ [ M(P).__dumpstate_array_avx2
+ : buf=_buf /\ offset=_off /\ lEN=_len /\ st=_st
+ /\ 0 <= _len <= 200
+ /\ to_uint _off + _len <= aSIZE
+ ==> res.`1 = A.fill (fun i=> (stbytes (stavx2_to_st25 _st)).[i-to_uint _off]) (to_uint _off) _len _buf
+  /\ res.`2 = _off + W64.of_int _len
+ ] = 1%r.
+proof.
+by conseq dumpstate_array_avx2_ll (dumpstate_array_avx2_h _buf _off _len _st).
+qed.
+*)
+
+phoare squeeze_array_avx2x4_ll: 
+ [ M(P).__squeeze_array_avx2x4
+ : 0 < rATE8 <= 200
+ ==> true
+ ] = 1%r.
+admitted.
+
+(*
+hoare squeeze_array_avx2_h _buf _off _len _st _r8:
+ M(P).__squeeze_array_avx2
+ : buf=_buf /\ offset=_off /\ lEN=_len /\ st=_st /\ rATE8=_r8
+ /\ 0 <= _len
+ /\ 0 < _r8 <= 200
+ /\ to_uint _off + _len <= aSIZE
+ ==> res.`1 = A.fill (fun i=> (SQUEEZE1600 _r8 _len (stavx2_to_st25 _st)).[i-to_uint _off]) (to_uint _off) _len _buf
+  /\ res.`2 = stavx2_from_st25 (st_i (stavx2_to_st25 _st) ((_len-1) %/ _r8 + 1)).
+proof.
+admitted.
+
+
+phoare squeeze_array_avx2_ph _buf _off _len _st _r8:
+ [ M(P).__squeeze_array_avx2
+ : buf=_buf /\ offset=_off /\ lEN=_len /\ st=_st /\ rATE8=_r8
+ /\ 0 <= _len
+ /\ 0 < _r8 <= 200
+ /\ to_uint _off + _len <= aSIZE
+ ==> res.`1 = A.fill (fun i=> (SQUEEZE1600 _r8 _len (stavx2_to_st25 _st)).[i-to_uint _off]) (to_uint _off) _len _buf
+  /\ res.`2 = stavx2_from_st25 (st_i (stavx2_to_st25 _st) ((_len-1) %/ _r8 + 1))
+ ] = 1%r.
+proof.
+by conseq squeeze_array_avx2_ll (squeeze_array_avx2_h _buf _off _len _st _r8).
+qed.
+*)
+
+end KeccakArrayAvx2x4.
